
2D
	Parábola
	Elipse
	Hipérbola

3D
	Cono elíptico: $\frac{x^{2}}{a^{2}}+\frac{y^{2}}{b^{2}}-\frac {z^{2}}{c^{3}}=0$
	 ![[Pasted image 20240210134935.png|200]]
	 Elipsoide: $\frac{x^{2}}{a^{2}}+\frac{y^{2}}{b^{2}}+\frac {z^{2}}{c^{3}}=1$
	  ![[Pasted image 20240210134914.png|200]]
	  Hiperboloide de 1 hoja: $\frac{x^{2}}{a^{2}}+\frac{y^{2}}{b^{2}}-\frac {z^{2}}{c^{3}}=1$
	  ![[Pasted image 20240210135139.png|200]]
	  Hiperboloide de 2 hojas: $-\frac{x^{2}}{a^{2}}-\frac{y^{2}}{b^{2}}+\frac {z^{2}}{c^{3}}=1$
	  ![[Pasted image 20240210135302.png|200]]
	  Paraboloide elíptico: $z=\frac{x^{2}}{a^{2}}+\frac{y^{2}}{b^{2}}$ 
	  ![[Pasted image 20240210135518.png|200]]
	  Paraboloide hiperbólico: $z=\frac{x^{2}}{a^{2}}-\frac{y^{2}}{b^{2}}$
	  ![[Pasted image 20240210135648.png|200]]
	  Cilindro elíptico: $\frac{y^{2}}{b^{2}}+\frac {z^{2}}{c^{3}}=1$ 
	  ![[Pasted image 20240210135925.png|200]]
	  Cilindro hiperbólico: $\frac{y^{2}}{b^{2}}-\frac {z^{2}}{c^{3}}=1$
	  ![[Pasted image 20240210140125.png|200]]
	  Cilindro parabólico: $y^{2}= b^{2}x^{2}$
	  ![[Pasted image 20240210140435.png|200]]
	  